Given_Clause_Loops/Prover_Lazy_List_Queue.thy
@@ -9,10 +9,38 @@ text \<open>This section covers the to-do data structure that arises in the
 Zipperposition loop.\<close>
 
 theory Prover_Lazy_List_Queue
-  imports Ordered_Resolution_Prover.Lazy_List_Chain
+  imports Prover_Queue
 begin
 
 
-subsection \<open>Setup and Basic Lemmas\<close>
+subsection \<open>Locales\<close>
+
+locale prover_llist_queue =
+  fixes
+    empty :: 'q and
+    add_llist :: "'e llist \<Rightarrow> 'q \<Rightarrow> 'q" and
+    pick_elem :: "'q \<Rightarrow> 'e \<times> 'q" and
+    remove_llist :: "'e llist \<Rightarrow> 'q \<Rightarrow> 'q" and
+    llists :: "'q \<Rightarrow> 'e llist multiset"
+  assumes
+    llists_empty[simp]: "llists empty = {#}" and
+    llists_not_empty[simp]: "P \<noteq> empty \<Longrightarrow> felems P \<noteq> {||}" and
+(*
+  fixes
+    empty :: "'p" and
+    select :: "'p \<Rightarrow> 'f" and
+    add :: "'f \<Rightarrow> 'p \<Rightarrow> 'p" and
+    remove :: "'f \<Rightarrow> 'p \<Rightarrow> 'p" and
+    felems :: "'p \<Rightarrow> 'f fset"
+  assumes
+    felems_empty[simp]: "felems empty = {||}" and
+    felems_not_empty[simp]: "P \<noteq> empty \<Longrightarrow> felems P \<noteq> {||}" and
+    select_in_felems[simp]: "P \<noteq> empty \<Longrightarrow> select P |\<in>| felems P" and
+    felems_add[simp]: "felems (add C P) = {|C|} |\<union>| felems P" and
+    felems_remove[simp]: "felems (remove C P) = felems P |-| {|C|}" and
+    add_again: "C |\<in>| felems P \<Longrightarrow> add C P = P"
+*)
+begin
+
 
 end
